Mica/TinyML.lean
@@ -5,7 +5,6 @@ import Mica.TinyML.Heap
 import Mica.TinyML.Untyped
 import Mica.TinyML.Typed
 import Mica.TinyML.OpSem
-import Mica.TinyML.LogicalRelation
 import Mica.TinyML.WeakestPre
 import Mica.TinyML.Typing
 import Mica.TinyML.Printer
